completeness is hard to prove...

coq/Mono.v
@@ -1,6 +1,11 @@
-Require Import Coq.Strings.String CoqRecon.Util.
+Require Import Coq.Strings.String
+        CoqRecon.Util Coq.Arith.PeanoNat.
 
 Instance StringEqDec : EqDec string eq := {equiv_dec := string_dec}.
+(*Instance NatEquiv : Equivalence eq := Nat.eq_equiv.*)
+Instance NatEqDec
+  : @EqDec nat (@eq nat) (@eq_equivalence nat) :=
+  {equiv_dec := Nat.eq_dec}.
 
 Inductive typ : Set :=
 | TBool
@@ -25,8 +30,57 @@ Fixpoint tvars (t : typ) : list nat :=
 Definition Ctvars : list (typ * typ) -> list nat :=
   fold_right (fun '(l,r) acc => tvars l ++ tvars r ++ acc) [].
 
+Definition tenv : Set := @env nat typ.
+
+Reserved Notation "s † t" (at level 20, right associativity).
+
+Fixpoint tsub (σ : tenv) (t : typ) {struct t} : typ :=
+  match t with
+  | TBool => TBool
+  | TNat => TNat
+  | (t → t')%typ => (σ † t → σ † t')%typ
+  | TVar T => match σ T with
+             | Some τ => τ
+             | None => TVar T
+             end
+  end
+where "σ † t" := (tsub σ t) : typ_scope.
+
+Lemma tsub_empty : forall t, (∅%env † t)%typ = t.
+Proof.
+  intro t; induction t; simpl in *; auto.
+  rewrite IHt1. rewrite IHt2. reflexivity.
+Qed.
+
+Lemma tsub_exists : forall t σ, exists τ σ', (σ' † t = σ † σ' † τ)%typ.
+Proof.
+  intro t; induction t as [| | t IHt t' IHt' | n]; intros s.
+  - exists TBool; exists ∅%env; reflexivity.
+  - exists TNat; exists ∅%env; reflexivity.
+  - specialize IHt with s; specialize IHt' with s. simpl.
+    destruct IHt as [t1 [s1 IHt1]]; destruct IHt' as [t2 [s2 IHt2]].
+    (*exists (s1 † t1 → s2 † t2)%typ.
+  - destruct (env_binds n s) as [Hns | [t Hns]].
+    + exists (TVar n); simpl; rewrite Hns; reflexivity.
+    + *)
+Abort.
+
+Notation "s1 ‡ s2"
+  := (fun t => (s1 † s2 † t)%typ)
+       (at level 21, left associativity).
+
+Definition satisfy σ τ1 τ2 : Prop := (σ † τ1 = σ † τ2)%typ.
+
 Inductive op : Set :=
 | And | Or | Add | Sub | Eq | Lt.
+
+Inductive op_typs : op -> typ -> typ -> Prop :=
+| ot_and : op_typs And TBool TBool
+| ot_or  : op_typs Or  TBool TBool
+| ot_add : op_typs Add TNat  TNat
+| ot_sub : op_typs Sub TNat  TNat
+| ot_eq  : op_typs Eq  TNat  TBool
+| ot_lt  : op_typs Lt  TNat  TBool.
 
 Inductive term : Set :=
 | Var : string -> term
@@ -34,8 +88,8 @@ Inductive term : Set :=
 | App : term -> term -> term
 | Bool : bool -> term
 | Nat : nat -> term
-| Cond : term -> term -> term
-| Op : op -> term -> term.
+| Cond : term -> term -> term -> term
+| Op : op -> term -> term -> term.
 
 Declare Scope term_scope.
 Delimit Scope term_scope with term.
@@ -48,6 +102,72 @@ Notation "e1 ⋅ e2"
        (at level 34, left associativity) : term_scope.
 
 Definition gamma : Set := @env string typ.
+
+Reserved Notation "g ⊨ e ∈ t" (at level 70).
+
+Inductive typing (Γ : gamma) : term -> typ -> Prop :=
+| t_bool b :
+    Γ ⊨ Bool b ∈ TBool
+| t_nat n :
+    Γ ⊨ Nat n ∈ TNat
+| t_var x τ :
+    bound x τ Γ ->
+    Γ ⊨ Var x ∈ τ
+| t_abs x e τ τ' :
+    (x ↦ τ;; Γ)%env ⊨ e ∈ τ' ->
+    Γ ⊨ (λ x ⇒ e)%term ∈ (τ → τ')%typ
+| t_app e1 e2 τ τ' :
+    Γ ⊨ e1 ∈ (τ → τ')%typ ->
+    Γ ⊨ e2 ∈ τ ->
+    Γ ⊨ (e1 ⋅ e2)%term ∈ τ'
+| t_cond e1 e2 e3 τ :
+    Γ ⊨ e1 ∈ TBool ->
+    Γ ⊨ e2 ∈ τ ->
+    Γ ⊨ e3 ∈ τ ->
+    Γ ⊨ Cond e1 e2 e3 ∈ τ
+| t_op o e1 e2 τ τ' :
+    op_typs o τ τ' ->
+    Γ ⊨ e1 ∈ τ ->
+    Γ ⊨ e2 ∈ τ ->
+    Γ ⊨ Op o e1 e2 ∈ τ'
+where "g ⊨ e ∈ t" := (typing g e t).
+
+Notation "s × g" := (env_map (tsub s) g)
+                      (at level 25, right associativity) : env_scope.
+
+Lemma tsub_gamma_empty : forall g : gamma, (∅ × g = g)%env.
+Proof.
+  intros g. extensionality n.
+  unfold env_map.
+  destruct (g n) eqn:Heq; auto.
+  rewrite tsub_empty. reflexivity.
+Qed.
+
+Section Prez.
+  Local Hint Constructors op_typs : core.
+
+  Lemma pres_op_typs : forall o τ τ',
+      op_typs o τ τ' ->
+      forall σ, op_typs o (σ † τ)%typ (σ † τ')%typ.
+  Proof.
+    intros o t t' H s; inv H; simpl; auto.
+  Qed.
+
+  Local Hint Resolve pres_op_typs : core.
+  Local Hint Constructors typing : core.
+  
+  Theorem preservation : forall Γ e τ,
+    Γ ⊨ e ∈ τ -> forall σ,
+      (σ × Γ)%env ⊨ e ∈ (σ † τ)%typ.
+  Proof.
+    intros g e t H;
+      induction H; intros s; simpl in *; eauto.
+    - constructor. unfold bound, env_map in *.
+      rewrite H. reflexivity.
+    - constructor.
+      rewrite env_map_bind; auto.
+  Qed.
+End Prez.
 
 Reserved Notation "g ⊢ e ∈ t ⊣ X @ C" (at level 70).
 
@@ -72,6 +192,162 @@ Inductive constraint_typing (Γ : gamma)
     Γ ⊢ e1 ∈ τ1 ⊣ X1 @ C1 ->
     Γ ⊢ e2 ∈ τ2 ⊣ X2 @ C2 ->
     Γ ⊢ (e1 ⋅ e2)%term ∈ TVar T
-      ⊣ (T :: X1 ++ X2) @ ((τ1, (τ2 → TVar T)%typ) :: C1 ++ C2)
+      ⊣ (T :: X1 ∪ X2)%set
+      @ ((τ1, (τ2 → TVar T)%typ) :: C1 ∪ C2)%set
+| ct_cond e1 e2 e3 τ1 τ2 τ3 X1 X2 X3 C1 C2 C3 :
+    (X1 ∩ X2)%set = [] ->
+    (X1 ∩ X3)%set = [] ->
+    (X2 ∩ X3)%set = [] ->
+    Γ ⊢ e1 ∈ τ1 ⊣ X1 @ C1 ->
+    Γ ⊢ e2 ∈ τ2 ⊣ X2 @ C2 ->
+    Γ ⊢ e3 ∈ τ3 ⊣ X3 @ C3 ->
+    Γ ⊢ Cond e1 e2 e3 ∈ τ2
+      ⊣ (X1 ∪ X2 ∪ X3)%set
+      @ ((τ1,TBool) :: (τ2,τ3) :: C1 ∪ C2 ∪ C3)%set
+| ct_op o e1 e2 τ1 τ2 τ τ' X1 X2 C1 C2 :
+    (X1 ∩ X2)%set = [] ->
+    op_typs o τ τ' ->
+    Γ ⊢ e1 ∈ τ1 ⊣ X1 @ C1 ->
+    Γ ⊢ e2 ∈ τ2 ⊣ X2 @ C2 ->
+    Γ ⊢ Op o e1 e2 ∈ τ'
+      ⊣ (X1 ∪ X2)%set
+      @ ((τ,τ1) :: (τ,τ2) :: C1 ∪ C2)%set
 where "g ⊢ e ∈ t ⊣ X @ C"
         := (constraint_typing g e t X C).
+
+Fail Fixpoint cgen (g : gamma) (e : term)
+  : typ * list nat * list (typ * typ) :=
+  match e with
+  | Var x => _
+  end.
+
+Section Sound.
+  Local Hint Constructors op_typs : core.
+  Local Hint Constructors typing : core.
+  Local Hint Resolve preservation : core.
+  Local Hint Resolve pres_op_typs : core.
+  
+  Theorem sound : forall Γ e t X C,
+    Γ ⊢ e ∈ t ⊣ X @ C ->
+    forall σ,
+      Forall (uncurry (satisfy σ)) C ->
+      (σ × Γ)%env ⊨ e ∈ (σ † t)%typ.
+  Proof.
+    intros g e t X C H; induction H; intros s HC; eauto.
+    - apply IHconstraint_typing in HC.
+      constructor. fold tsub.
+      rewrite <- env_map_bind in HC.
+      assumption.
+    - inv HC. rewrite Forall_app in H8.
+      destruct H8 as [HC1 HC2].
+      unfold uncurry, satisfy in H7.
+      apply IHconstraint_typing1 in HC1.
+      apply IHconstraint_typing2 in HC2.
+      rewrite H7 in HC1. eauto.
+    - inv HC. inv H8.
+      repeat rewrite Forall_app in H10.
+      destruct H10 as [[HC1 HC2] HC3].
+      apply IHconstraint_typing1 in HC1.
+      apply IHconstraint_typing2 in HC2.
+      apply IHconstraint_typing3 in HC3.
+      unfold uncurry, satisfy in *; simpl in *.
+      rewrite H7 in HC1. rewrite <- H9 in HC3. auto.
+    - inv HC. inv H6.
+      rewrite Forall_app in H8.
+      destruct H8 as [HC1 HC2].
+      apply IHconstraint_typing1 in HC1.
+      apply IHconstraint_typing2 in HC2.
+      unfold uncurry,satisfy in *.
+      rewrite <- H5 in HC1; rewrite <- H7 in HC2. eauto.
+  Qed.
+End Sound.
+
+Section Complete.
+  Local Hint Resolve sound : core.
+  Local Hint Resolve preservation : core.
+  
+  Lemma gamma_map : forall (g : gamma) (s : tenv) T t,
+      s T = None ->
+      (T ↦ t;; s × g = T ↦ t;; ∅ × s × g)%env.
+  Proof.
+    intros g s T t HsT. extensionality n.
+    unfold env_map, bind.
+    destruct (g n) as [tn |] eqn:Hgn;
+      try reflexivity; f_equal.
+    clear Hgn g n.
+    generalize dependent T;
+      generalize dependent t;
+      generalize dependent s.
+    induction tn as [| | t1 IHt1 t2 IHt2 | m];
+      intros s t T HsT; simpl; try reflexivity.
+    - rewrite IHt1, IHt2 by assumption; reflexivity.
+    - destruct (equiv_dec m T) as [HmT | HmT];
+        unfold equiv, complement in *; subst.
+      + rewrite HsT. simpl.
+        destruct (equiv_dec T T) as [? | ?];
+          unfold equiv, complement in *;
+          try contradiction; try reflexivity.
+      + destruct (s m) as [tm |] eqn:Hsm; simpl.
+        * clear m s HsT HmT Hsm.
+          induction tm; simpl; try reflexivity.
+          -- rewrite <- IHtm1; rewrite <- IHtm2.
+             reflexivity.
+          -- destruct (equiv_dec n T) as [HnT | HnT];
+               unfold equiv, complement in *; simpl;
+                 try reflexivity. admit.
+        * destruct (equiv_dec m T) as [? | ?];
+            unfold equiv, complement in *;
+            try contradiction; try reflexivity.
+  Admitted.
+  
+  Theorem complete : forall Γ e t X C,
+    Γ ⊢ e ∈ t ⊣ X @ C ->
+    forall σ τ d,
+      (σ × Γ)%env ⊨ e ∈ τ ->
+      dom σ d -> (X ∩ d = [])%set ->
+      exists σ', Forall (uncurry (satisfy σ')) C /\
+            (σ † t = τ)%typ /\ (σ' ∉ X = σ)%env.
+  Proof.
+    intros g e τ X C H; induction H;
+      intros s t d Ht Hd Hemp. (*inv Ht.*)
+    - inv Ht; exists s; intuition.
+    - inv Ht; exists s; intuition.
+    - inv Ht; exists s; intuition.
+      unfold bound,env_map in *.
+      rewrite H in H1. inv H1.
+      reflexivity.
+    - inv Ht.
+      assert
+        (((T ↦ ((T ↦ τ0;; ∅)%env † τ0)%typ;; s) × x ↦ TVar T;; Γ)
+           %env ⊨ e ∈ ((T ↦ τ0;; ∅)%env † τ')%typ).
+      { assert (s T = None).
+        { assert (~ In T d).
+          { intros HIn.
+            apply In_member in HIn. simpl in Hemp.
+            rewrite HIn in Hemp; simpl in *.
+            discriminate. }
+          eauto using not_in_dom. }
+        apply preservation
+          with (σ := (T ↦ τ0;; ∅)%env) in H4.
+        rewrite <- env_map_bind.
+        unfold tsub at 1. rewrite bind_sound.
+        rewrite <- env_map_bind in H4.
+        Check gamma_map.
+        
+        
+        
+  (* apply preservation
+        with (σ := (T ↦ τ0;; ∅)%env) in H4.
+      (*Set Printing Implicit.
+      Set Typeclasses Debug.    *)
+      remember (T ↦ ((T ↦ τ0;; ∅)%env † τ0)%typ;; s)%env as s' eqn:Heqs'.
+      remember ((T ↦ τ0;; ∅)%env † τ')%typ as t' eqn:Heqt'.
+      specialize IHconstraint_typing
+        with (d := T :: d) (σ := s') (τ0 := t').
+      subst s'; subst t'.
+      rewrite <- env_map_bind in H4.
+      rewrite <- env_map_bind in IHconstraint_typing.
+      unfold tsub at 1 in IHconstraint_typing.
+      rewrite bind_sound in IHconstraint_typing. *)
+  Admitted.
+End Complete.
